Define durable state of inode

src/program_proof/examples/inode_proof.v
@@ -1,5 +1,7 @@
 From RecordUpdate Require Import RecordSet.
 
+From Perennial.goose_lang Require Import crash_modality.
+
 From Goose.github_com.mit_pdos.perennial_examples Require Import dir.
 From Perennial.program_proof Require Import proof_prelude.
 
@@ -8,8 +10,9 @@ From Perennial.program_proof Require Import marshal_proof.
 
 Module inode.
   Record t :=
-    mk { blocks: list Block; }.
-  Global Instance _eta: Settable _ := settable! mk <blocks>.
+    mk { addr: u64;
+         blocks: list Block; }.
+  Global Instance _eta: Settable _ := settable! mk <addr; blocks>.
   Global Instance _witness: Inhabited t := populate!.
   Definition size σ := length σ.(blocks).
 End inode.
@@ -21,18 +24,40 @@ Context `{!lockG Σ}.
 Let inodeN := nroot.@"inode".
 
 Implicit Types (σ: inode.t).
+Implicit Types (l:loc) (γ:gname) (P: inode.t → iProp Σ).
 
 Definition inode_linv (l:loc) σ : iProp Σ :=
-  ∃ (addr: u64) (addr_s: Slice.t) (addrs: list u64) (hdr: Block),
-    ⌜Block_to_vals hdr = b2val <$> encode ([EncUInt64 (U64 $ length addrs)] ++ (map EncUInt64 addrs))⌝ ∗
-    int.val addr d↦ hdr ∗
-    l ↦[inode.S :: "addr"] #addr ∗
-    l ↦[inode.S :: "addrs"] (slice_val addr_s) ∗
-    is_slice addr_s uint64T 1 addrs ∗
+  ∃ (addr_s: Slice.t) (addrs: list u64) (hdr: Block),
+    "%Hencoded" ∷ ⌜Block_to_vals hdr = b2val <$> encode ([EncUInt64 (U64 $ length addrs)] ++ (map EncUInt64 addrs))⌝ ∗
+    "Hhdr" ∷ int.val σ.(inode.addr) d↦ hdr ∗
+    "addr" ∷ l ↦[inode.S :: "addr"] #σ.(inode.addr) ∗
+    "addrs" ∷ l ↦[inode.S :: "addrs"] (slice_val addr_s) ∗
+    "Haddrs" ∷ is_slice addr_s uint64T 1 addrs ∗
     (* TODO: this does not support reading lock-free; we could make it [∃ q,
     int.val a d↦{q} b], but that wouldn't support lock-free writes if we
     implemented those *)
-    [∗ list] a;b ∈ addrs;σ.(inode.blocks), int.val a d↦ b
+    "Hdata" ∷ [∗ list] a;b ∈ addrs;σ.(inode.blocks), int.val a d↦ b
 .
+
+Definition is_inode l γ P : iProp Σ :=
+  ∃ (d:val) (lref: loc), "d" ∷ readonly (l ↦[inode.S :: "d"] d) ∗
+                         "m" ∷ readonly (l ↦[inode.S :: "m"] #lref) ∗
+                         "Hlock" ∷ is_lock inodeN γ #lref (∃ σ, inode_linv l σ ∗ P σ).
+
+Definition is_inode_durable σ : iProp Σ :=
+  ∃ (addrs: list u64) (hdr: Block),
+    "%Hencoded" ∷ ⌜Block_to_vals hdr = b2val <$> encode ([EncUInt64 (U64 $ length addrs)] ++ (map EncUInt64 addrs))⌝ ∗
+    "Hhdr" ∷ int.val σ.(inode.addr) d↦ hdr ∗
+    "Hdata" ∷ [∗ list] a;b ∈ addrs;σ.(inode.blocks), int.val a d↦ b.
+
+Theorem is_inode_crash l σ :
+  IntoCrash (inode_linv l σ) (λ _, is_inode_durable σ).
+Proof.
+  hnf; iIntros "Hinv".
+  iNamed "Hinv".
+  iExists addrs, hdr.
+  iFrame "% ∗".
+  auto.
+Qed.
 
 End goose.
